src/Init/Data/String/Pattern/Basic.lean
@@ -285,26 +285,24 @@ where
 
 @[inline]
 def memcmpSlice (lhs rhs : Slice) (lstart : String.Pos.Raw) (rstart : String.Pos.Raw)
-    (len : String.Pos.Raw) (h1 : len.offsetBy lstart ≤ lhs.rawEndPos)
-    (h2 : len.offsetBy rstart ≤ rhs.rawEndPos) : Bool :=
+    (len : String.Pos.Raw) (h1 : len.offsetBy lstart ≤ lhs.endExclusive.offset)
+    (h2 : len.offsetBy rstart ≤ rhs.endExclusive.offset) : Bool :=
   memcmpStr
     lhs.str
     rhs.str
-    (lstart.offsetBy lhs.startInclusive.offset)
-    (rstart.offsetBy rhs.startInclusive.offset)
+    lstart
+    rstart
     len
-    (by
-      have := lhs.startInclusive_le_endExclusive
-      have := lhs.endExclusive.isValid.le_utf8ByteSize
-      simp [String.Pos.le_iff, Pos.Raw.le_iff, Slice.utf8ByteSize_eq,
-        -String.Pos.byteIdx_offset_le_utf8ByteSize] at *
-      omega)
-    (by
-      have := rhs.startInclusive_le_endExclusive
-      have := rhs.endExclusive.isValid.le_utf8ByteSize
-      simp [String.Pos.le_iff, Pos.Raw.le_iff, Slice.utf8ByteSize_eq,
-        -String.Pos.byteIdx_offset_le_utf8ByteSize] at *
-      omega)
+    (Pos.Raw.le_iff.2 (by
+      have h₁ := Pos.Raw.le_iff.1 h1
+      have h₂ := lhs.endExclusive.isValid.le_utf8ByteSize
+      simp only [Pos.Raw.byteIdx_offsetBy, String.byteIdx_rawEndPos] at h₁ ⊢
+      omega))
+    (Pos.Raw.le_iff.2 (by
+      have h₁ := Pos.Raw.le_iff.1 h2
+      have h₂ := rhs.endExclusive.isValid.le_utf8ByteSize
+      simp only [Pos.Raw.byteIdx_offsetBy, String.byteIdx_rawEndPos] at h₁ ⊢
+      omega))
 
 end Internal
 
